\item[15.] $y'' + 3y'- 4y= e^{3t}, y_0 = y_0' = 0$
\begin{gather*}
    L(y'')=p^2Y-py_0-y_0';\:
    L(y')=pY-y_0;\:
    L(y)=Y;\:\\
    L(y'' + 3y'- 4y)=(p^2Y-py_0-y_0')+3(pY-y_0)-4(Y)\\
    L(y'' + 3y'- 4y)=p^2Y+3pY-4Y=(p+4)(p-1)Y\\
    (p+4)(p-1)Y=L(e^{3t}) \implies Y=\frac{1}{(p+4)(p-1)}\cdot L(e^{3t})\\
\end{gather*}
\begin{equation*}
    L^{-1}\Bigg(\frac{1}{(p+4)(p-1)} \Bigg) 
    = \frac{e^{-(-1)t}-e^{-(4)t}}{4-(-1)}=\frac{e^{t}-e^{-4t}}{5}
    \tag{By \( L7 \)}
\end{equation*}
\begin{align*}
    y 
    & = \int^t_0 \frac{e^{\tau}-e^{-4\tau}}{5}e^{3(t-\tau)}d\tau\\
    & = \frac{e^{3t}}{5}\int^t_0 (e^{\tau}-e^{-4\tau})e^{-3\tau}d\tau\\
    & = \frac{e^{3t}}{5}\int^t_0 e^{-2\tau}-e^{-7\tau}d\tau\\
    & = \frac{e^{3t}}{5}\Big( \frac{1}{7}e^{-7\tau}-\frac{1}{2}e^{-2\tau}\Big)\Big|^t_0\\
    & = \frac{e^{3t}}{5}
    \Bigg(
    \Big( \frac{1}{7}e^{-7t}-\frac{1}{2}e^{-2t}\Big)
    -\Big( \frac{1}{7}e^{-7(0)}-\frac{1}{2}e^{-2(0)}\Big)
    \Bigg)\\
    & = \frac{e^{3t}}{5}
    \Big(\frac{1}{7}e^{-7t}-\frac{1}{2}e^{-2t} + \frac{5}{14}\Big)\\
    & = \textcolor{red}{\frac{1}{35}e^{-4t}-\frac{1}{10}e^{t} + \frac{1}{14}e^{3t}}
\end{align*}