\item[14.] $y'' + 5y'+ 6y= e^{-2t}, y_0 = y_0' = 0$
\begin{gather*}
    L(y'')=p^2Y-py_0-y_0';\:
    L(y')=pY-y_0;\:
    L(y)=Y;\:\\
    L(y'' + 5y'+ 6y)=(p^2Y-py_0-y_0')+5(pY-y_0)+6(Y)\\
    L(y'' + 5y'+ 6y)=p^2Y+5pY+6Y=(p+2)(p+3)Y\\
    (p+2)(p+3)Y=L(e^{2t}) \implies Y=\frac{1}{(p+2)(p+3)}\cdot L(e^{2t})\\
\end{gather*}
\begin{equation*}
    L^{-1}\Bigg(\frac{1}{(p+2)(p+3)} \Bigg) 
    = \frac{e^{-(3)t}-e^{-(2)t}}{2-(3)}=e^{-2t}-e^{-3t}
    \tag{By \( L7 \)}
\end{equation*}
\begin{align*}
    y 
    & = \int^t_0 (e^{-2\tau}-e^{-3\tau})e^{-2(t-\tau)}d\tau\\
    & = e^{-2t}\int^t_0 (e^{-2\tau}-e^{-3\tau})e^{2\tau}d\tau\\
    & = e^{-2t}\int^t_0 1-e^{-\tau}d\tau\\
    & = e^{-2t}(\tau+e^{-\tau})\Big|^t_0\\
    & = e^{-2t}\Big((t+e^{-t})-(0+e^{-0}\Big)\\
    & = e^{-2t}(t+e^{-t}-1)\\
    & = \textcolor{red}{te^{-2t}+e^{-3t}-e^{-2t}}\\
\end{align*}