\item[4.]$\frac{1}{(p+a)(p+b)^2}$
\[
    \frac{1}{(p+a)(p+b)^2} = \frac{1}{(p+a)}\cdot\frac{1}{(p+b)^2}
\]
\begin{equation*}
    L^{-1}\Bigg(\frac{1}{(p+a)}\Bigg) 
    = e^{-at}
    \tag{By \( L2 \)}
\end{equation*}
\begin{equation*}
    L^{-1}\Bigg(\frac{1}{(p+b)^2}\Bigg) 
    = te^{-bt}
    \tag{By \( L6 \)}
\end{equation*}
\begin{align*}
    L^{-1}\Bigg( \frac{1}{(p+a)(p+b)^2} \Bigg)
    & = \int_0^t e^{-a(t-\tau)} \tau e^{-b\tau}d\tau \\
    & = \int_0^t \tau e^{-a(t-\tau)-b\tau}d\tau \\
    & = \int_0^t \tau e^{-at+(a-b)\tau}d\tau \\
    & = e^{-at}\int_0^t \tau e^{(a-b)\tau}d\tau \\
    & = e^{-at}\Bigg(\Big(\frac{\tau e^{(a-b)\tau}}{(a-b)}
    \Big)\Bigg|_0^t-\frac{1}{(a-b)} \int_0^t e^{(a-b)\tau}d\tau \Bigg)\\
    & = e^{-at}\Bigg(\frac{\tau e^{(a-b)\tau}}{(a-b)}
    -\frac{e^{(a-b)\tau}}{(a-b)^2}   \Bigg)\Bigg|_0^t\\
    & = e^{-at}\Bigg(
    \Big(\frac{t e^{(a-b)t}}{(a-b)}
    -\frac{e^{(a-b)t}}{(a-b)^2}\Big)
    -\Big(0
    -\frac{e^{(a-b)0}}{(a-b)^2}\Big)
    \Bigg)\\
    & = e^{-at}\Bigg(
    \frac{(a-b)t e^{(a-b)t}-e^{(a-b)t}+1}{(a-b)^2}
    \Bigg)\\
    & = \textcolor{red}{\frac{(a-b)t e^{-bt}-e^{-bt}+e^{-at}}{(a-b)^2}}\\
\end{align*}