\item[9.]$\frac{2}{p^3(p+2)}$
\[
    \frac{2}{p^3(p+2)} = \frac{2}{p^3}\cdot\frac{1}{p+2}
\]
\begin{equation*}
    L^{-1}\Bigg(\frac{2}{p^3}\Bigg) 
    = t^2
    \tag{By \( L5 \)}
\end{equation*}
\begin{equation*}
    L^{-1}\Bigg(\frac{1}{p+2}\Bigg) 
    = e^{-2t}
    \tag{By \( L2 \)}
\end{equation*}
\begin{align*}
    L^{-1}\Bigg( \frac{2}{p^3(p+2)} \Bigg)
    & = \int_0^t \tau^2e^{-2(t-\tau)} d\tau \\
    & =e^{-2t} \int_0^t \tau^2e^{2\tau} d\tau \\
    & =e^{-2t}\Bigg(\frac{\tau^2e^{2\tau}}{2}\Big|^t_0 -\int_0^t \tau e^{2\tau} d\tau \Bigg)\\
    & =e^{-2t}\Bigg(\Big(\frac{\tau^2e^{2\tau}}{2}-\frac{\tau e^{2\tau}}{2}\Big)\Big|^t_0 +\frac{1}{2}\int_0^t e^{2\tau} d\tau \Bigg)\\
    & =e^{-2t}\Bigg(\frac{\tau^2e^{2\tau}}{2}-\frac{\tau e^{2\tau}}{2} +\frac{e^{2\tau}}{4} \Bigg)\Bigg|^t_0\\
    & =e^{-2t}\Bigg(
    \Big(\frac{t^2e^{2t}}{2}-\frac{t e^{2t}}{2} +\frac{e^{2t}}{4} \Big)
    -\Big(\frac{(0)^2e^{2(0)}}{2}-\frac{(0) e^{2(0)}}{2} +\frac{e^{2(0)}}{4} \Big)
    \Bigg)\\
    & =e^{-2t}\Bigg(
    \frac{t^2e^{2t}}{2}-\frac{t e^{2t}}{2} +\frac{e^{2t}}{4} 
    -\frac{1}{4} \Bigg)\\
    & =\textcolor{red}{
    \frac{t^2}{2}-\frac{t}{2} +\frac{1}{4} 
    -\frac{e^{-2t}}{4}}
\end{align*}