\item [12.] $y''-y= e^{-t}-2te^{-t}$, $y_0=1$, $y_0'=2$
\begin{gather*}
    L(y'')=p^2Y-py_0-y_0';\:
    L(y')=pY-y_0;\:
    L(y)=Y;\:
    L(e^{-t}-2te^{-t})=\frac{1}{p+1}-\frac{2}{(p+1)^2}
\end{gather*}
\begin{align*}
    y''- y
    &=p^2Y-py_0-y_0'-(Y)\\
    &=p^2Y-p(1)-(2)-Y\\
    &=p^2Y-p-2-Y\\
    &=p^2Y-Y-p-2\\
    &=(p+1)(p-1)Y-p-2
\end{align*}
\begin{gather*}
    (p+1)(p-1)Y-p-2=\frac{1}{p+1}-\frac{2}{(p+1)^2}\\
    Y=\frac{\frac{1}{p+1}-\frac{2}{(p+1)^2}+p+2}{(p+1)(p-1)}
    =\frac{\frac{p-1}{(p+1)^2}+p+2}{(p+1)(p-1)}
    =\frac{1}{(p+1)^3}+\frac{p+2}{(p+1)(p-1)}
\end{gather*}
Using Partial Fraction Decomp:
\begin{gather*}
    \frac{p+2}{(p+1)(p-1)}=\frac{A}{p+1}+\frac{B}{p-1}\\
    \implies A(p-1)+B(p+1) = p+2
    \implies (A+B)p+(-A+B) = p+2\\
    \implies A+B = 1 \text { and }-A+B = 2
    \implies A+A+2 = 1 \implies A = -1/2 \implies B = 3/2\\
    \frac{p+2}{(p+1)(p-1)}=\frac{-1/2}{p+1}+\frac{3/2}{p-1}
\end{gather*}
\begin{gather*}
    Y=\frac{1}{(p+1)^3}+\frac{-1/2}{p+1}+\frac{3/2}{p-1}
\end{gather*}
\begin{equation*}
    L^{-1}\Bigg(\frac{1}{(p+1)^3}\Bigg) 
    = \frac{1}{2}L^{-1}\Bigg(\frac{(2)!}{(p+(1))^{(2)+1}}\Bigg) 
    =\frac{1}{2}t^{(2)} e^{-(1)t}
    =\frac{1}{2}t^2e^{-t}
    \tag{By \( L6 \)}
\end{equation*}
\begin{equation*}
    L^{-1}\Bigg(\frac{-1/2}{p+1}\Bigg) 
    = -\frac{1}{2}L^{-1}\Bigg(\frac{1}{p+(1)}\Bigg) 
    =-\frac{1}{2}e^{-(1)t}
    =-\frac{1}{2}e^{-t}
    \tag{By \( L2 \)}
\end{equation*}
\begin{equation*}
    L^{-1}\Bigg(\frac{3/2}{p-1}\Bigg) 
    = \frac{3}{2}L^{-1}\Bigg(\frac{1}{p+(-1)}\Bigg) 
    =\frac{3}{2}e^{-(-1)t}
    =\frac{3}{2}e^{t}
    \tag{By \( L2 \)}
\end{equation*}
\textcolor{red}{\[
   y= \frac{1}{2}t^2e^{-t}-\frac{1}{2}e^{-t}+\frac{3}{2}e^{t}
\]}