\item [7.] $y''- 4y' + 4y= 4$, $y_0=0$, $y_0'=-2$
\begin{gather*}
    L(y'')=p^2Y-py_0-y_0';\:
    L(y')=pY-y_0;\:
    L(y)=Y;\:
    L(4)=4/p
\end{gather*}
\begin{align*}
    y''- 4y' + 4y
    &=p^2Y-py_0-y_0'-4(pY-y_0)+4(Y)\\
    &=p^2Y-p(0)-(-2)-4(pY-(0))+4Y\\
    &=p^2Y+2-4pY+4Y\\
    &=p^2Y-4pY+4Y+2\\
    &=(p-2)^2Y+2
\end{align*}
\begin{gather*}
    (p-2)^2Y+2=\frac{4}{p}\\
    Y=\frac{4-2p}{p(p-2)^2}=\frac{-2}{p(p-2)}
\end{gather*}
Using partial fraction decomposition
\begin{gather*}
    Y=\frac{A}{p}+\frac{B}{p-2} \text{ s.t. } A(p-2)+Bp =  -2\\
    \implies (A+B)p-2A = -2 \text{ so } A  = 1\\
    \implies (1+B)p = 0 \text{ so } B  = -1\\
    Y=\frac{1}{p}-\frac{1}{p-2}
\end{gather*}
\begin{equation*}
    L^{-1}\Bigg(\frac{1}{p}\Bigg) 
    =1
    \tag{By \( L1 \)}
\end{equation*}
\begin{equation*}
    L^{-1}\Bigg(-\frac{1}{p-2}\Bigg) 
    = -L^{-1}\Bigg(\frac{1}{p+(-2)}\Bigg) 
    =-e^{-(-2)t}
    =-e^{2t}
    \tag{By \( L2 \)}\\
\end{equation*}
\textcolor{red}{\[
   y= 1-e^{2t}
\]}