\item[11.] $\frac{2z-i}{iz+2}$
\begin{align*}
    f(z) 
    &= \frac{2z-i}{iz+2} \\
    &= \frac{2(x+iy)-i}{i(x+iy)+2} \\
    &= \frac{2x+2iy-i}{ix+i^2y+2} \\
    &= \frac{2x+2iy-i}{ix-y+2} \\
    &= \frac{2x+2iy-i}{ix-y+2} \frac{ix+y-2}{ix+y-2}\\
    &= \frac{(2x+2iy-i)(ix+y-2)}{(ix-y+2)(ix+y-2)} \\
    &= \frac{2ix^2+2i^2xy-i^2x+2xy+2iy^2-iy-4x-4iy+2i}{(ix)^2-(y-2)^2} \\
    &= \frac{-3x+2ix^2+2iy^2-5iy+2i}{-x^2-(y-2)^2} \\
    &= \frac{3x-2ix^2-2iy^2+5iy-2i}{x^2+(y-2)^2} \\
    &= \frac{3x}{x^2+(y-2)^2} +i\frac{-2x^2-2y^2+5y-2}{x^2+(y-2)^2}
\end{align*}
\[
\boxed{
\answer{
\begin{aligned}
u(x,y) &= \frac{3x}{x^2+(y-2)^2} \\
v(x,y) &= \frac{-2x^2-2y^2+5y-2}{x^2+(y-2)^2}
\end{aligned}
}
}
\]
