\item[12.] $\frac{z}{z^2+1}$
\begin{align*}
    f(z) 
    &= \frac{z}{z^2+1} \\
    &= \frac{x+iy}{(x+iy)^2+1}\\
    &= \frac{x+iy}{x^2+2xiy+(iy)^2+1}\\
    &= \frac{x+iy}{x^2-y^2+1+2xiy}\\
    &= \frac{x+iy}{x^2-y^2+1+2xiy}\frac{x^2-y^2+1-2xiy}{x^2-y^2+1-2xiy}\\
    &= \frac{x^3-xy^2+x-2x^2iy+x^2yi-iy^3+iy-2x(iy)^2}{(x^2-y^2+1)^2-(2xiy)^2}\\
    &= \frac{x^3+x+xy^2-x^2iy-iy^3+iy}{(x^2-y^2+1)^2+(2xy)^2}\\
    &= \frac{x^3+x+xy^2}{(x^2-y^2+1)^2+(2xy)^2}+i\frac{-x^2y-y^3+y}{(x^2-y^2+1)^2+(2xy)^2}
\end{align*}
\[
\boxed{
\answer{
\begin{aligned}
u(x,y) &= \frac{x^3+x+xy^2}{(x^2-y^2+1)^2+(2xy)^2} \\
v(x,y) &= \frac{-x^2y-y^3+y}{(x^2-y^2+1)^2+(2xy)^2}
\end{aligned}
}
}
\]
