\item[11.] $\frac{2z-i}{iz+2}$
\begin{align*}
    u(x,y) &= \frac{3x}{x^2+(y-2)^2} \\
    v(x,y) &= \frac{-2x^2-2y^2+5y-2}{x^2+(y-2)^2}
\end{align*}
\begin{align*}
    \pd{u}{x}  
    &= \frac{(3)(x^2+(y-2)^2)-(3x)(2x)}{(x^2+(y-2)^2)^2} \\
    &= \frac{3x^2+3(y-2)^2-6x^2}{(x^2+(y-2)^2)^2} \\
    &= \frac{-3x^2+3y^2-12y+12}{(x^2+(y-2)^2)^2} \\
    \pd{v}{y}  
    &= \frac{(-4y+5)(x^2+(y-2)^2)-(-2x^2-2y^2+5y-2)(2(y-2))}{(x^2+(y-2)^2)^2} \\
    &= \frac{(-4y+5)(x^2+(y-2)^2)-(-4x^2y-4y^3+10y^2-4y)+(-8x^2-8y^2+20y-8)}{(x^2+(y-2)^2)^2} \\
    &= \frac{(-4y+5)(x^2+(y-2)^2)+4x^2y+4y^3-10y^2+4y-8x^2-8y^2+20y-8}{(x^2+(y-2)^2)^2} \\
    &= \frac{(-4y+5)(x^2+(y-2)^2)+4x^2y+4y^3-18y^2+24y-8x^2-8}{(x^2+(y-2)^2)^2} \\
    &= \frac{-4x^2y+-4y(y-2)^2+5x^2+5(y-2)^2+4x^2y+4y^3-18y^2+24y-8x^2-8}{(x^2+(y-2)^2)^2} \\
    &= \frac{-4y(y-2)^2+5(y-2)^2+4y^3-18y^2+24y-3x^2-8}{(x^2+(y-2)^2)^2} \\
    &= \frac{-4y(y-2)^2+4y^3-13y^2+4y-3x^2+12}{(x^2+(y-2)^2)^2} \\
    &= \frac{-3x^2+3y^2-12y+12}{(x^2+(y-2)^2)^2} \\
    \pd{u}{y}  
    &= \frac{(0)(x^2+(y-2)^2)-(3x)(2(y-2))}{(x^2+(y-2)^2)^2} \\
    &= \frac{-6xy+12x}{(x^2+(y-2)^2)^2} \\
\end{align*}
\begin{align*}
    \pd{v}{x}  
    &= \frac{(-4x)(x^2+(y-2)^2-(-2x^2-2y^2+5y-2)(2x)}{(x^2+y^2)^2} \\
    &= \frac{-4x^3-4xy^2+16xy-16x+4x^3+4xy^2-10xy+4x}{(x^2+y^2)^2} \\
    &= \frac{16xy-16x-10xy+4x}{(x^2+y^2)^2} \\
    &= \frac{6xy-12x}{(x^2+y^2)^2} \\
\end{align*}
\answer{
Since $\pd{u}{x} = \pd{v}{y}$ and $-\pd{u}{y} = \pd{v}{x}$, $f(z) = \frac{2z-i}{iz+2}$ is analytical (assuming $z \neq 2i$).
}
