\item[12.] $\frac{z}{z^2+1}$
\begin{align*}
    u(x,y) &= \frac{x^3 + x + x y^2}{(x^2 - y^2 + 1)^2 + 4x^2 y^2} \\
    v(x,y) &= \frac{-x^2 y - y^3 + y}{(x^2 - y^2 + 1)^2 + 4x^2 y^2}
\end{align*}
\begin{align*}
    \pd{u}{x} &= \frac{-x^6-x^4y^2-x^4+x^2y^4-10x^2y^2+x^2+y^6-y^4-y^2+1}{\left(x^4+2x^2y^2+2x^2+y^4-2y^2+1\right)^2} \\
    \pd{v}{y} &= \frac{y^6+y^4x^2-y^4-y^2x^4-10y^2x^2-y^2-x^6-x^4+x^2+1}{\left(y^4+2y^2x^2-2y^2+x^4+2x^2+1\right)^2} \\
    \pd{u}{y} &= \frac{2y^5x+4y^3x^3+4y^3x+2yx^5-4yx^3-6yx}{\left(y^4+2y^2x^2-2y^2+x^4+2x^2+1\right)^2} \\
    \pd{v}{x} &= \frac{-2x^5y-4x^3y^3+4x^3y-2xy^5-4xy^3+6xy}{\left(x^4+2x^2y^2+2x^2+y^4-2y^2+1\right)^2}
\end{align*}
\answer{
Since $\pd{u}{x} = \pd{v}{y}$ and $-\pd{u}{y} = \pd{v}{x}$, $f(z) = \frac{2z-i}{iz+2}$ is analytical (assuming $z \neq \pm i$).
}


