\item[55.] $3x^2y - y^3$\\
\[
\frac{\partial^2 u}{\partial x^2} = \frac{\partial}{\partial x}(6xy) = 6y, \quad 
\frac{\partial^2 u}{\partial y^2} = \frac{\partial}{\partial y}(-3y^2) = -6y \quad \Rightarrow \quad \answer{\Delta u = 6y - 6y = 0}
\]
Thus, $u$ is harmonic.
\[
\frac{\partial u}{\partial x} = 6xy = \frac{\partial v}{\partial y}, \quad 
\frac{\partial u}{\partial y} = 3x^2 - 3y^2 = -\frac{\partial v}{\partial x}
\]
\[
\frac{\partial v}{\partial y} = 6xy \Rightarrow v = 3xy^2 + g(x), \quad
-\frac{\partial v}{\partial x} = 3x^2 - 3y^2 \Rightarrow \frac{\partial v}{\partial x} = -3x^2 + 3y^2
\]

Take the derivative of \( v = 3xy^2 + g(x) \) with respect to \( x \):
\[
\frac{\partial v}{\partial x} = 3y^2 + g'(x) = -3x^2 + 3y^2 \Rightarrow g'(x) = -3x^2
\Rightarrow g(x) = -x^3 + C
\]

Thus,
\[
v(x, y) = 3xy^2 - x^3 + C
\]
For this question we choose $C = 0$
\answer{\[
f(z) =3x^2y - y^3 + i(3xy^2 - x^3)
\]}
\[
\frac{\partial^2 v}{\partial x^2} = \frac{\partial}{\partial x}(-3x^2 + 3y^2) = -6x, \quad 
\frac{\partial^2 v}{\partial y^2} = \frac{\partial}{\partial y}(6xy) = 6x \quad \Rightarrow \quad \answer{\Delta v = -6x + 6x = 0}
\]
Thus, $v$ is harmonic.