\item [16.] Solve the differential equation $yy'^2 + 2xy' - y = 0$ by changing from variables $y$, $x$, to $r$, $x$, where $y^2= r^2 - x^2$; then $yy'= rr' - x$.
\begin{gather*}
    yy'^2 + 2xy' - y = 0\\
    y^2y'^2 + 2xyy' - y^2 = 0\\
    y^2y'^2 + 2xyy' +x^2 - y^2 - x^2 = 0\\
    (yy' + x)^2 - (y^2 + x^2) = 0\\
    (rr')^2 - r^2 = 0\\
    r'^2 - 1 = 0\\
    r' = \pm 1 \\
    \int r' dx = \int \pm 1 dx\\
    r = \pm x + C\\
    r^2 = x^2 \pm 2xC + C^2\\
    r^2 - x^2 = \pm 2xC + C^2\\
    y^2 = \pm 2xC + C^2\\
    \textcolor{red}{
    y = \sqrt{\pm 2xC + C^2}
    }
\end{gather*}