\item [Example 1] $y''+y'-2y=0$

\begin{gather*}
    (D^2+D-2)y=0\\
    \text{Auxillary Equation: }(D^2+D-2)=0\\
    \implies (D+2)(D-1)=0 \implies \text{root(s): }-2,1\\
    \text{General Solution: } y=C_1e^{-2x}+C_2e^x
\end{gather*}

\item [Example 2] $4y''+12y'+9y=0$

\begin{gather*}
    (4D^2+12D+9)y=0\\
    \text{Auxillary Equation: }(4D^2+12D+9)=0\\
    \implies (2D+3)^2=0 \implies \text{root(s):}-\frac{3}{2}\\
    \text{General Solution: } y=e^{-\frac{3}{2}x}(Ax+B)
\end{gather*}


% pg 406, section 4: 16
% pg 414, section 5: 1,2,5,8,10,12