\item [2.] $P_2(x)$ on $(-1,1)$\vspace{-5mm}
\begin{gather*}
    \norm{P_2(x)} 
    = \sqrt{\innerproduct{P_2(x)}{P_2(x)}}
    = \sqrt{\int_{-1}^1 (P_2(x))^2dx}
    = \sqrt{\int_{-1}^{1} \Big(\frac{1}{2}(3x^2-1)\Big)^2dx}\\
    = \sqrt{\frac{1}{4}\int_{-1}^{1} (9x^4-6x^2+1)dx}
    = \sqrt{\frac{1}{4} \Big(\frac{9}{5}x^5-2x^3+x\Big)\Big|_{-1}^{1}}\\
    = \sqrt{\frac{1}{4} 
    \Big[
    \Big(\frac{9}{5}(1)^5-2(1)^3+(1)\Big)
    -
    \Big(\frac{9}{5}(-1)^5-2(-1)^3+(-1)\Big)
    \Big]
    }\\
    = \sqrt{\frac{1}{2} 
    \Big(\frac{9}{5}-2+1\Big)
    }
    = \sqrt{\frac{1}{2} 
    \Big(\frac{4}{5}\Big)
    }
    = \answer{\sqrt{\frac{2}{5}}}
\end{gather*}
\begin{gather*}
    \frac{P_2(x)}{\norm{P_2(x)}} 
    = \frac{\frac{1}{2}(3x^2-1)}{\sqrt{2/5}}
    = \answer{\frac{\sqrt{5}}{2\sqrt{2}}(3x^2-1)}
\end{gather*}