\item [1.] $\displaystyle f(x) = 
\begin{cases}
    -1, & -1 < x < 0\\
    \:\:\,\,1, & \:\:\,\,0 < x < 1\\
\end{cases}$\\[5mm]
Observe that
\[
    \int_{-1}^1f(x)P_l(x)dx =
    \begin{cases}
        0, & l \text{ is even}\\
        2 \int_0^1 P_l(x)dx, & l \text{ is odd}
    \end{cases}
\]
\begin{gather*}
    \int_{-1}^{1}f(x)P_0(x)dx =C_0\cdot \frac{2}{2(0)+1} = 2C_0\\
    \int_{-1}^{1}f(x)P_0(x)dx = 0\\
    2C_0 = 0 \implies \answer{C_0 = 0}
\end{gather*}
\begin{gather*}
    \int_{-1}^{1}f(x)P_1(x)dx =C_1\cdot \frac{2}{2(1)+1} = \frac{2}{3}C_1\\
    \int_{-1}^{1}f(x)P_1(x)dx 
    = 2\int_0^1 x dx = x^2\big|_0^1 = 1\\
    \frac{2}{3}C_1 = 1 \implies \answer{C_1 = \frac{3}{2}}
\end{gather*}
\begin{gather*}
    \int_{-1}^{1}f(x)P_2(x)dx =C_2\cdot \frac{2}{2(2)+1} = \frac{2}{5}C_2\\
    \int_{-1}^{1}f(x)P_2(x)dx = 0\\
    \frac{2}{5}C_2 = 0 \implies \answer{C_2 = 0}
\end{gather*}
\begin{gather*}
    \int_{-1}^{1}f(x)P_3(x)dx =C_0\cdot \frac{2}{2(3)+1} = \frac{2}{7}C_3\\
    \int_{-1}^{1}f(x)P_3(x)dx 
    = 2\int_0^1 \frac{1}{2}(5x^3-3x) dx 
    = \int_0^1 (5x^3-3x) dx
    = \frac{5}{4}x^4-\frac{3}{2}x^2\big|_0^1 
    = -\frac{1}{4}\\
    \frac{2}{7}C_3 = -\frac{1}{4} \implies \answer{C_3 = -\frac{7}{8}}
\end{gather*}
\begin{gather*}
    \int_{-1}^{1}f(x)P_4(x)dx =C_4\cdot \frac{2}{2(4)+1} = \frac{2}{9}C_4\\
    \int_{-1}^{1}f(x)P_4(x)dx = 0\\
    \frac{2}{9}C_4 = 0 \implies \answer{C_4 = 0}
\end{gather*}
The Legendre series for this function is:
\answer{
\[
    \frac{3}{2}P_1(x)-\frac{7}{8}P_3(x)+...
\]
}