\item [3.] $f(x)= P_3'(x)$
\[
    P_3'(x) = (\frac{5}{2}x^3 - \frac{3}{2}x)' = \frac{15}{2}x^2 - \frac{3}{2}
\]
Observe that
\[
    \int_{-1}^1f(x)P_l(x)dx =
    \begin{cases}
        0, & l \text{ is odd}\\
        2 \int_{0}^1 (\frac{15}{2}x^2 - \frac{3}{2})P_l(x)dx, & l \text{ is even}
    \end{cases}
\]
\begin{gather*}
    \int_{-1}^{1}f(x)P_0(x)dx =C_0\cdot \frac{2}{2(0)+1} = 2C_0\\
    \int_{-1}^{1}f(x)P_0(x)dx 
    = 2 \int_0^1 \frac{15}{2}x^2 - \frac{3}{2} dx 
    = 5x^3 - 3x\Big|_0^1 
    = 2\\
    2C_0 = 2 \implies \answer{C_0 = 1}
\end{gather*}
\begin{gather*}
    \int_{-1}^{1}f(x)P_1(x)dx =C_1\cdot \frac{2}{2(1)+1} = \frac{2}{3}C_1\\
    \int_{-1}^{1}f(x)P_1(x)dx = 0\\
    \frac{2}{3}C_1 = 0 \implies \answer{C_1 = 0}
\end{gather*}
\begin{gather*}
    \int_{-1}^{1}f(x)P_2(x)dx =C_2\cdot \frac{2}{2(2)+1} = \frac{2}{5}C_2\\
    \int_{-1}^{1}f(x)P_2(x)dx
    = 2 \int_0^1 \Big(\frac{15}{2}x^2 - \frac{3}{2}\Big)
    \Big(\frac{3}{2}x^2 - \frac{1}{2}\Big)dx \\
    = \int_0^1 \frac{45}{2}x^4-12x^2+\frac{3}{2}dx
    = \frac{9}{2}x^5-4x^3+\frac{3}{2}x\Big|_0^1 
    = 2\\
    \frac{2}{5}C_2 = 2 \implies \answer{C_2 = 5}
\end{gather*}
\begin{gather*}
    \int_{-1}^{1}f(x)P_3(x)dx =C_0\cdot \frac{2}{2(3)+1} = \frac{2}{7}C_3\\
    \int_{-1}^{1}f(x)P_3(x)dx 
    = 0\\
    \frac{2}{7}C_3 = 0 \implies \answer{C_3 = 0}
\end{gather*}
\begin{gather*}
    \int_{-1}^{1}f(x)P_4(x)dx =C_4\cdot \frac{2}{2(4)+1} = \frac{2}{9}C_4\\
    \int_{-1}^{1}f(x)P_4(x)dx
    = 2 \int_0^1 \Big(\frac{15}{2}x^2 - \frac{3}{2}\Big)
    \Big(\frac{35}{8}x^4 - \frac{30}{8}x^2 + \frac{3}{8}\Big)dx \\
    = \frac{1}{8}\int_0^1 525x^6-555x^4+135x^2-9 dx 
    = \frac{1}{8}\Big(75x^7-111x^5+45x^3-9\Big)\Big|_0^1 
    = 0\\
    \frac{2}{9}C_4 = 0 \implies \answer{C_4 = 0}
\end{gather*}
The Legendre series for this function is:
\answer{
\[
    P_0(x)+
    5P_2(x)+
    ...
\]
}