\item [4.] $(D+1)(D-3)y=24e^{-3x}$\\[2mm]
First Find General Solution to homogeneous equation:
\begin{gather*}
    \text{Auxiliary Equation: } (D+1)(D-3)=0 \implies \text{root(s): } -1,3\\
    \text{General Solution: } y_c=Ae^{-x}+Be^{3x}
\end{gather*}
Now Find particular Solution:
Using a simple way to solve for the particular solution we know $y_p=Ce^{-3x}$
% \begin{gather*}
%     (D+1)(D-3)y_p = 24e^{-3x} \text{; Let }u = (D-3)y_p\\
%     (D+1)u = 24e^{3x} \implies u' + u = 24e^{-3x}\\
%     I(x) = \int dx = x \text{ and } Q(x) = 24e^{-3x}\\
%     u = e^{-x}\int e^{x}24e^{-3x}dx = -12e^{3x}\\
%     y_p'-3y_p=-12e^{3x}\\
%     I(x) = \int -3dx = -3x \text{ and } Q(x) = -12e^{-3x}\\
%     y_p = e^{3x}\int e^{-3x}(-12)e^{-3x}dx = 2e^{-3x}\\
% \end{gather*}
\begin{gather*}
    y_p=Ce^{-3x};\:y_p'=C(-3)e^{-3x};\:y_p''=C9e^{-3x}\\
    y_p''-2y_p'-3y_p=C\big((9e^{-3x})-2((-3)e^{-3x})-3(e^{-3x})\big)\\
    y_p''-2y_p'-3y_p=12Ce^{-3x} = 24e^{-3x} \text{ so } C=2\\
    y_p = 2e^{-3x}
\end{gather*}
Combine:
\begin{gather*}
    y=y_c+y_p\\
    \textcolor{red}{y = Ae^{-x}+Be^{3x}+2e^{-3x}}
\end{gather*}