\item [5.] $(D^2+1)y=2e^{x}$\\[2mm]
First Find General Solution to homogeneous equation:
\begin{gather*}
    \text{Auxiliary Equation: } (D+i)(D-i)=0 \implies \text{root(s): } \pm i\\
    \text{General Solution: } y_c=Ae^{-ix}+Be^{ix}
\end{gather*}
Now Find particular Solution:
Using a simple way to solve for the particular solution we know $y_p=Ce^{x}$
% \begin{gather*}
%     (D+i)(D-i)y_p = 2e^{x} \text{; Let }u = (D-i)y_p\\
%     (D+i)u = 2e^{x} \implies u' + iu = 2e^{x}\\
%     I(x) = \int idx = ix \text{ and } Q(x) = 2e^{x}\\
%     u = e^{-ix}\int e^{ix}2e^{x}dx = \frac{2}{(1+i)}e^{x}\\
%     y_p'-3y_p=\frac{2}{(1+i)}e^{x}\\
%     I(x) = \int -idx = -ix \text{ and } Q(x) = \frac{2}{(1+i)}e^{x}\\
%     y_p = e^{ix}\int e^{-ix}\frac{2}{(1+i)}e^{x}dx = \frac{2}{(1+i)(1-i)}e^{x}=e^x\\
% \end{gather*}
\begin{gather*}
    y_p=Ce^{x};\:y_p'=Ce^{x};\:y_p''=Ce^{x}\\
    y_p''+y_p=C\big((e^{x})+(e^{x})\big)\\
    y_p''+y_p=2Ce^{x} = 2e^{x} \text{ so } C=1\\
    y_p = e^{x}
\end{gather*}
Combine:
\begin{gather*}
    y=y_c+y_p\\
    \textcolor{red}{y = Ae^{-ix}+Be^{ix}+e^x}
\end{gather*}