\item [6.] $y''+6y'+9y=12e^{-x}$\\[2mm]
First Find General Solution to homogeneous equation:
\begin{gather*}
    \text{Auxiliary Equation: } (D+3)^2=0 \implies \text{root(s): } -3\\
    \text{General Solution: } y_c=(Ax+B)e^{-3x}
\end{gather*}
Now Find particular Solution:
Using a simple way to solve for the particular solution we know $y_p=Ce^{-x}$
% \begin{gather*}
%     (D+3)^2y_p = 12e^{-x} \text{; Let }u = (D+3)y_p\\
%     (D+3)u = 12e^{-x} \implies u' + 3u = 12e^{-x}\\
%     I(x) = \int 3dx = 3x \text{ and } Q(x) = 12e^{-x}\\
%     u = e^{-3x}\int e^{3x}12e^{-x}dx = 6e^{-x}\\
%     y_p'+3y_p=6e^{-x}\\
%     I(x) = \int 3dx = 3x \text{ and } Q(x) = 6e^{-x}\\
%     y_p = e^{-3x}\int e^{3x}6e^{-x}dx = 3e^{-x}\\
% \end{gather*}
\begin{gather*}
    y_p=Ce^{-x};\:y_p'=-Ce^{-x};\:y_p''=Ce^{-x}\\
    y_p''+6y_p'+9y_p=C\big((e^{-x})+6(-e^{-x})+9(e^{x})\big)\\
    y_p''+6y_p'+9y_p=4Ce^{-x} = 12e^{-x} \text{ so } C=3\\
    y_p = 3e^{-x}
\end{gather*}
Combine:
\begin{gather*}
    y=y_c+y_p\\
    \textcolor{red}{y = (Ax+B)e^{-3x}+3e^{-x}}
\end{gather*}