\item [7.] $y''-y'-2y=3e^{2x}$\\[2mm]
First Find General Solution to homogeneous equation:
\begin{gather*}
    \text{Auxiliary Equation: } (D+1)(D-2)=0 \implies \text{root(s): } -1,2\\
    \text{General Solution: } y_c=Ae^{-x}+Be^{2x}
\end{gather*}
Now Find particular Solution:\\
Because exponent on RHS is one of the roots of the auxiliary equation, particular solution in the form of $Cxe^{2x}$
\begin{gather*}
    y_p=Cxe^{2x};\:y_p'=C(e^{2x}+2xe^{2x});\:y_p''=C(4e^{2x}+4xe^{2x})\\
    y_p''-y_p'-2y_p=C\big((4e^{2x}+\cancel{4xe^{2x}})-(e^{2x}+\cancel{2xe^{2x}})-\cancel{2(xe^{2x})}\big)\\
    y_p''-y_p'-2y_p=3Ce^{2x} = 3e^{2x} \text{ so } C=1\\
    y_p = xe^{2x}
\end{gather*}
Combine:
\begin{gather*}
    y=y_c+y_p\\
    \textcolor{red}{y = Ae^{-x}+Be^{2x}+xe^{2x}}
\end{gather*}