\item [9.] $(D^2+2D+1)y=2e^{-x}$\\[2mm]
First Find General Solution to homogeneous equation:
\begin{gather*}
    \text{Auxiliary Equation: } (D+1)^2=0 \implies \text{root(s): } -1\\
    \text{General Solution: } y_c=(Ax+B)e^{-x}
\end{gather*}
Now Find particular Solution:\\
Because exponent on RHS is the same as both roots of the auxiliary equation, particular solution in the form of $Cx^2e^{-x}$
\begin{gather*}
    y_p=Cx^2e^{-x};\:y_p'=C(2xe^{-x}-x^2e^{-x});\:y_p''=C(2e^{-x}-4xe^{-x}+x^2e^{-x})\\
    y_p''+2y_p'+y_p\\=C\big(
        (2e^{-x}-\cancel{4xe^{-x}}+\cancel{x^2e^{-x}})
        +\cancel{2(2xe^{-x}-x^2e^{-x})}
        +\cancel{(x^2e^{-x})}
    \big)\\
    =2Ce^{-x} = 2e^{-x} \text{ so } C=1\\
    y_p = x^2e^{-x}
\end{gather*}
Combine:
\begin{gather*}
    y=y_c+y_p\\
    \textcolor{red}{y = (Ax+B+x^2)e^{-x}}
\end{gather*}