\item [2.]$y'-y=2e^t$, $y_0=3$
\begin{gather*}
    L(y')=pY-y_0;\: L(y)=Y;\: L(2e^t)=\frac{2}{p-1}\\
    y'-y=pY-y_0-Y=pY-3-Y = (p-1)Y-3=\frac{2}{p-1}\\
    Y = \frac{2}{(p-1)^2}+\frac{3}{p-1}
\end{gather*}
\begin{equation*}
    L^{-1}\Bigg(\frac{2}{(p-1)^2}\Bigg) 
    = 2L^{-1}\Bigg(\frac{(1)!}{(p+(-1))^{(1)+1}}\Bigg)
    =2t^{(1)}e^{-(-1)t}=2te^t
    \tag{By \( L6 \)}
\end{equation*}
\begin{equation*}
    L^{-1}\Bigg(\frac{3}{p-1}\Bigg)
    = 3L^{-1}\Bigg(\frac{1}{p+(-1)}\Bigg)
    =3e^{-(-1)t}=3e^t 
    \tag{By \( L2 \)}
\end{equation*}

\begin{gather*}
    y=L^{-1}(Y)=L^{-1}
    \Bigg(
    \frac{2}{(p-1)^2}+\frac{3}{p-1}
    \Bigg)=\textcolor{red}{2te^t+3e^t}
\end{gather*}

