\item [4.] $y''+y=\sin t$, $y_0=1$, $y_0'=0$
\begin{gather*}
    L(y'')=p^2Y-py_0-y_0';\:
    L(y')=pY-y_0;\:
    L(y)=Y;\:
    L(\sin t)=\frac{1}{p^2+1}
\end{gather*}
\begin{align*}
    y''+y
    &=p^2Y-py_0-y_0'+Y\\
    &=p^2Y-p(1)-(0)+Y\\
    &=p^2Y-p+Y\\
    &=(p^2+1)Y-p
\end{align*}
\begin{gather*}
    (p^2+1)Y-p=\frac{1}{p^2+1}\\
    Y=\frac{1}{(p^2+1)^2}+\frac{p}{p^2+1}
\end{gather*}
\begin{gather*}
    L^{-1}\Bigg(\frac{1}{(p^2+1)^2}\Bigg) 
    = \frac{1}{2}L^{-1}\Bigg(\frac{2(1)^3}{(p^2+1^2)^2}\Bigg) 
    =\frac{1}{2}(\sin((1)t) - (1)t \cos((1)t))\\
    =\frac{1}{2}\sin(t) - \frac{1}{2}t\cos(t)
    \tag{By \( L17 \)}
\end{gather*}
\begin{equation*}
    L^{-1}\Bigg(\frac{p}{p^2+1}\Bigg) 
    = L^{-1}\Bigg(\frac{p}{p^2+1^2}\Bigg)
    = \cos((1)t)
    =\cos(t)
    \tag{By \( L4 \)}
\end{equation*}
\textcolor{red}{\[
   y= \frac{1}{2}\sin(t) - \frac{1}{2}t\cos(t)+\cos(t)
\]}