\item [6.] $y''- 6y' + 9y= te^{3t}$, $y_0=0$, $y_0'=5$
\begin{gather*}
    L(y'')=p^2Y-py_0-y_0';\:
    L(y')=pY-y_0;\:
    L(y)=Y;\:
    L(te^{3t})=\frac{1}{(p-3)^2}
\end{gather*}
\begin{align*}
    y''- 6y' + 9y
    &=p^2Y-py_0-y_0'-6(pY-y_0)+9(Y)\\
    &=p^2Y-p(0)-(5)-6(pY-(0))+9Y\\
    &=p^2Y-5-6pY+9Y\\
    &=p^2Y-6pY+9Y-5\\
    &=(p-3)^2Y-5
\end{align*}
\begin{gather*}
    (p-3)^2Y-5=\frac{1}{(p-3)^2}\\
    Y=\frac{1}{(p-3)^4}+\frac{5}{(p-3)^2}
\end{gather*}
\begin{equation*}
    L^{-1}\Bigg(\frac{1}{(p-3)^4}\Bigg) 
    = \frac{1}{6}L^{-1}\Bigg(\frac{(3)!}{(p+(-3))^{(3)+1}}\Bigg) 
    =\frac{1}{6}t^{(3)}e^{-(-3)t}
    =\frac{1}{6}t^3e^{3t}
    \tag{By \( L6 \)}
\end{equation*}
\begin{equation*}
    L^{-1}\Bigg(\frac{5}{(p-3)^3}\Bigg) 
    = 5L^{-1}\Bigg(\frac{(1)!}{(p+(-3))^{(1)+1}}\Bigg) 
    =5t^{(1)}e^{-(-3)t}
    =5te^{3t}
    \tag{By \( L6 \)}\\
\end{equation*}
\textcolor{red}{\[
   y= \frac{1}{6}t^3e^{3t}+5te^{3t}
\]}