\item $xy'=xy+y$
\begin{align*}
    y &= a_0 + a_1x + a_2x^2 + a_3x^3 + a_nx^n\\
    xy + y &= a_0 + (a_0 + a_1)x + (a_1 + a_2)x^2 + (a_2 + a_3)x^3 + (a_{n-1} + a_n)x^n \\
    y' &= a_1 + 2a_2x + 3a_3x^2 + 4a_4x^3 + na_nx^{n-1} \\
    xy' &= a_1x + 2a_2x^2 + 3a_3x^3 + na_nx^n \\
    a_0 &= 0 \\
    a_1 &= a_0 + a_1 = a_1 = a_1/0!\\
    2a_2 &= a_1 + a_2 \implies a_2 = a_1 = a_1/1!\\
    3a_3 &= a_2 + a_3 \implies a_3 = a_2/2 = a_1/2!\\
    4a_4 &= a_3 + a_4 \implies a_4 = a_3/3 = a_1/3!\\
\end{align*}
\[
a_n = 
\begin{cases}
    0 & n = 0\\
    \frac{a_1}{(n-1)!} & \text{otherwise}
\end{cases}
\]
\textcolor{red}{\[
    y 
    = \sum_{n=0}^\infty a_nx^n
    = \sum_{n=1}^\infty \frac{a_1x^n}{(n-1)!} 
    = a_1x\sum_{n=0}^\infty \frac{x^n}{n!} 
    = a_1xe^x
\]}