\item $y'=3x^2y$
\begin{align*}
    y &= a_0 + a_1x + a_2x^2 + a_3x^3 + a_nx^n\\
    3x^2y &= 3a_0x^2 + 3a_1x^3 + 3a_2x^4 + 3a_3x^5 + 3a_nx^{n+2}\\
    y' &= a_1 + 2a_2x + 3a_3x^2 + 4a_4x^3 + 5a_5x^4 + 6a_6x^5 + na_nx^{n-1} \\
    a_0 &= a_0 = a_0/0! \\
    a_1 &= 0\\
    2a_2 &= 0\\
    3a_3 &= 3a_0 \implies a_3 = a_0 = a_0/1!\\
    4a_4 &= 3a_1 \implies a_4 = 0\\
    5a_5 &= 3a_2 \implies a_5 = 0\\
    6a_6 &= 3a_3 \implies a_6 = a_3/2 = a_0/2!\\
\end{align*}
\[
a_n = 
\begin{cases}
    \frac{a_0}{(n/3)!} & \text{if $3$ divides }n\\
    0 & \text{otherwise}
\end{cases}
\]
\textcolor{red}{\[
    y 
    = \sum_{n=0}^\infty a_nx^n
    = \sum_{n=0}^\infty \frac{a_0x^{3n}}{n!} 
    = a_0\sum_{n=0}^\infty \frac{x^{3n}}{n!} 
    = a_0e^{x^3}
\]}