\item [4.] $\displaystyle \frac{d^{25}}{dx^{25}} (x\cos{x})$
\begin{align*}
    \frac{d^{25}}{dx^{25}} (x\cos{x})
    &= \sum_{k=0}^{25} \binom{25}{k}
    \frac{d^{k}}{dx^{k}} (x)
    \frac{d^{25-k}}{dx^{25-k}} (e^x)\\
    &= 
    \binom{25}{0}
    \frac{d^{0}}{dx^{0}} (x)
    \frac{d^{25-0}}{dx^{25-0}} (\cos{x})
    +
    \binom{25}{1}
    \frac{d^{1}}{dx^{1}} (x)
    \frac{d^{25-1}}{dx^{25-1}} (\cos{x})
    +
    \sum_{k=2}^{25} \binom{25}{k}
    \frac{d^{k}}{dx^{k}} (x)
    \frac{d^{25-k}}{dx^{25-k}} (e^x)\\
    &= 
    -x\sin{x}
    +
    25\cos{x}
    +
    0\\
    &= \textcolor{red}{-x\sin{x} + 25\cos{x}}
\end{align*}