\item $2y' = 3(y - 2)^{1/3}$, $y=3$ when $x=1$

\textcolor{blue}{
    \begin{minipage}[t]{0.45\textwidth}
        General Solution:
        \begin{gather*}
            2\frac{dy}{dx} = 3(y - 2)^{1/3}\\
            \frac{2}{3}\frac{1}{(y - 2)^{1/3}}dy =dx\\
            \frac{2}{3}\int\frac{1}{(y - 2)^{1/3}}dy=\int dx\\
            \frac{2}{3}\frac{3}{2}(y-2)^{2/3}=x+C\\
            \textcolor{red}{
            (y-2)^{2/3}=x+C
            }
        \end{gather*}
    \end{minipage}
    \hfill
    \begin{minipage}[t]{0.45\textwidth}
        Integration for LHS:\\
        $u=y-2$; $du=dy$
        \begin{gather*}
            \int\frac{1}{(y - 2)^{1/3}}dy=\int(u)^{-1/3}du\\
            \frac{3}{2}u^{2/3}+C=\frac{3}{2}(y-2)^{2/3}+C
        \end{gather*}
        Particular Solution:
        \begin{gather*}
            ((3)-2)^{2/3}=(1)+C\\
            1=1+C\\
            C=0\\
            \textcolor{red}{
                (y-2)^{2/3}=x
            }
        \end{gather*}
    \end{minipage}
}