\item $x\sqrt{1-y^2}dx+y\sqrt{1-x^2}dy=0$, $y = \frac{1}{2}$ when $x = \frac{1}{2}$
    
    \textcolor{blue}{
    \begin{minipage}[t]{0.45\textwidth}
        General Solution:
        \begin{gather*}
            x\sqrt{1-y^2}dx+y\sqrt{1-x^2}dy = 0 \\
            y\sqrt{1-x^2}dy = -x\sqrt{1-y^2}dx \\
            \frac{y}{\sqrt{1-y^2}}dy = -\frac{x}{\sqrt{1-x^2}}dx \\
            \int\frac{y}{\sqrt{1-y^2}}dy = -\int\frac{x}{\sqrt{1-x^2}}dx \\
            -\frac{1}{2}\sqrt{1-y^2} = \frac{1}{2}\sqrt{1-x^2}+C \\
            \frac{1}{2}\sqrt{1-y^2} + \frac{1}{2}\sqrt{1-x^2} = C \\
            \textcolor{red}{
            \sqrt{1-y^2} + \sqrt{1-x^2} = C   
            }
        \end{gather*}
    \end{minipage}
    \hfill
    \begin{minipage}[t]{0.45\textwidth}
        Integration:\\
            $u = 1-t^2$; $du = -2tdt$; $dt = -\frac{1}{2t}du$      
        \[
            \int\frac{t}{\sqrt{1-t^2}}dt =\int\frac{t}{\sqrt{u}}\frac{-1}{2t}du
        \]
        \[
            =-\frac{1}{2}\int\frac{1}{\sqrt{u}}du
            = -\frac{1}{2}(\sqrt{u})+C
        \]
        \[= -\frac{1}{2}\sqrt{1-t^2}+C\]
        Particular Solution:
        \begin{gather*}
            \sqrt{1-(1/2)^2} + \sqrt{1-(1/2)^2} = C \\
            C = \sqrt{3/4}+\sqrt{3/4} = \sqrt3 \\
            \textcolor{red}{
            \sqrt{1-y^2} + \sqrt{1-x^2} = \sqrt3
            }
        \end{gather*}
    \end{minipage}
    }