\item $y dy + (xy^2 - 8x) dx = 0$, $y=3$ when $x=1$

\textcolor{blue}{
    \begin{minipage}[t]{0.45\textwidth}
        General Solution:
        \begin{gather*}
            y dy + (xy^2 - 8x) dx = 0\\
            -y dy = (xy^2 - 8x) dx\\
            -y dy = x(y^2-8) dx\\
            -\frac{y}{y^2-8} dy = x dx\\
            -\int\frac{y}{y^2-8} dy = \int x dx\\
            -\frac{1}{2}\ln|y^2-8|=\frac{x^2}{2}+C\\
            \ln|y^2-8|=-x^2+C\\
            e^{\ln|y^2-8|}=e^{-x^2+C}\\
            \textcolor{red}{
            y^2-8=Ce^{-x^2}
            }
        \end{gather*}
    \end{minipage}
    \hfill
    \begin{minipage}[t]{0.45\textwidth}
        Integration for LHS:\\
        $u=y^2-8$; $du=2ydy$
        \begin{gather*}
            \int\frac{y}{y^2-8} dy = \frac{1}{2}\int\frac{1}{u} dy\\
            \frac{1}{2}\ln|u|+C=\frac{1}{2}\ln|y^2-8|+C
        \end{gather*}
        Particular Solution:
        \begin{gather*}
            (3)^2-8=Ce^{-(1)^2}\\
            9-8=C/e\\
            C=e\\
            \textcolor{red}{
                y^2-8=e \cdot e^{-x^2}
            }
        \end{gather*}
    \end{minipage}
}