\item [3.] Solve the semi-infinite plate problem if the bottom edge of width $\pi$ is held at $T = \cos{x}$ and the other sides are at 0\textdegree.\\[5mm]
Define the boundary constraints
\begin{align*}
    T(x,y=0)=\cos x\\
    T(x,y=\infty)=0\\
    T(x=0,y)=0\\
    T(x=\pi,y)=0
\end{align*}
Use $X(x)''+k^2X(x) = 0$ to get $X(x) = C_1\sin(kx)+C_2\cos(kx)$. Using the boundary constraints of $X(0) = 0$, $C_2 = 0$. Further from the constraint $X(\pi) = 0$, $k = n$ for all positive integers $n$ so 
\[\displaystyle X(x) = \sum_{n=1}^{\infty} C_n \sin\left(n x\right)\]
Next, use $Y(y)''-k^2Y(y)=0$ to get $Y(y) = Ae^{-ky}+Be^{ky}$. Because of the boundary constraint that as $y \rightarrow \infty$, $Y(y) = 0$, we know that $B = 0$ so $Y(y) = Ce^{-ky} = Ce^{-ny}$.\\[2mm]
Thus, as $T(x,y) = X(x)Y(y)$ we now have $\displaystyle T(x,y) = \sum_{n=1}^{\infty} C_n \sin\left(n x\right) e^{-ny}$\\[2mm]
To solve for $C_n$, we use \begin{align*}
    C_n &= \frac{2}{\pi} \int_0^{\pi} \cos(x)\sin\left(n x\right) dx \\
    &= \frac{2}{\pi} \int_0^{\pi} \frac{1}{2} [\sin(n x + x) + \sin(n x - x)] dx\\
    &= \frac{1}{\pi} \int_0^{\pi} \sin\big((n + 1)x\big) + \sin\big((n - 1) x\big) dx\\
    &= \frac{1}{\pi} \left[ \frac{-\cos\big((n + 1)x\big)}{n+1} + \frac{-\cos\big((n - 1)x\big)}{n-1} \right]_{0}^{\pi}\\
    &= \frac{1}{\pi} \left[ - \frac{\cos\big((n + 1)x\big)}{n+1} - \frac{\cos\big((n - 1)x\big)}{n-1} \right]_{0}^{\pi}\\
    &= \frac{1}{\pi} \left[ - \frac{\cos\big((n + 1)\pi\big)}{n+1} - \frac{\cos\big((n - 1)\pi\big)}{n-1} + \frac{\cos\big((n + 1)0\big)}{n+1} + \frac{\cos\big((n - 1)0\big)}{n-1}\right]\\
    &= \frac{1}{\pi} \left[ -\frac{(-1)^{n + 1}}{n+1} - \frac{(-1)^{n - 1}}{n-1} + \frac{1}{n+1} + \frac{1}{n-1}\right]\\
    &= \frac{1}{\pi} \left[ -\frac{(-1)^{n + 1}(n-1)}{(n+1)(n-1)} - \frac{(-1)^{n - 1}(n+1)}{(n+1)(n-1)} + \frac{n-1}{(n+1)(n-1)} + \frac{n+1}{(n+1)(n-1)}\right]\\
    &= \frac{1}{\pi} \left[ - \frac{(-1)^{n - 1}2n}{(n-1)(n+1)} + \frac{2n}{(n-1)(n+1)}\right]\\
    &= \frac{2n}{\pi} \left[ \frac{(-1)^{n}+1}{n^2-1} \right]
\end{align*}
Thus, when $n$ is even $C_n = \frac{4n}{\pi(n^2-1)}$ and when $n$ is odd $C_n = 0$.
Substituting this in we have
\answer{\[
    T(x,y) = \frac{4}{\pi}\sum_{\substack{n = 2 \\ \text{even } n}}^{\infty} \frac{n}{n^2-1} \sin\left(n x\right) e^{-ny}
\]}