\item [7.] $(1 + e^x)y' + 2e^xy = (1 + e^x)e^x$

\textcolor{blue}{
    \begin{gather*}
        y' + \frac{2e^x}{1 + e^x}y = e^x\\
        P(x)=\frac{2e^x}{1 + e^x}; \quad Q(x)=e^x\\
        I(x)=\int P(x)dx = \int \frac{2e^x}{1 + e^x}dx=2\ln|1+e^x|\\
        e^{-I(x)}=e^{-2\ln|1+e^x|}=(1+e^x)^{-2}\\
        \int e^{I(x)}Q(x)dx=\int e^{2\ln|1+e^x|}e^{x}dx=\int e^x(1+e^x)^{2}dx=\frac{1}{3}(1+e^x)^{3}+C\\
        y=e^{-I(x)}\int e^{I(x)}Q(x)dx=(1+e^x)^{-2}(\frac{1}{3}(1+e^x)^{3}+C)\\
        \textcolor{red}{
        y=\frac{1}{3}(1+e^x)+C(1+e^x)^{-2}
        }
    \end{gather*}
}